\documentclass{beamer}
\usepackage{xspace}

 \usepackage{calc}                                             %%
    \usepackage{multirow}                                         %%
    \usepackage{hhline}                                           %%
    \usepackage{ifthen}
\usetheme{CambridgeUS}

\title{Assignment 7:Papoulis Chapter 9}
\author{Saanvi Amrutha-AI21BTECH11026}
\date{\today}
\logo{\large \LaTeX{}}

\usepackage{amsmath}
\setbeamertemplate{caption}[numbered]{}
\providecommand{\pr}[1]{\ensuremath{\Pr\left(#1\right)}}
\providecommand{\cbrak}[1]{\ensuremath{\left\{#1\right\}}}
\providecommand{\brak}[1]{\ensuremath{\left(#1\right)}}
\begin{document}

\begin{frame}
    \titlepage 
\end{frame}

\logo{}

\begin{frame}{Outline}
    \tableofcontents
\end{frame}

\section{Question}
\begin{frame}{Question}
    \begin{block}{}
       Show that 
       \begin{enumerate} 
       \item if $R_x[m_1,m_2]= q[m_1]\delta[m_1 - m_2]$ and $s=\sum_{n=0}^N a_n x[n]$ then $E\cbrak{s^2}=\sum_{n=0}^N a_n^2q[n]$\\
       \item if $R_x\brak{t_1,t_2}=q\brak{t_1}\delta\brak{t_1-t_2}$ and $s=\int_{0}^{T}a\brak{t}x\brak{t}dt$ then 
       $E\cbrak{s^2}=\int_{0}^{T}a^2\brak{t}q\brak{t}dt$
       \end{enumerate}
    \end{block}
\end{frame}

\section{Solution}
\begin{enumerate}
\begin{frame}
\frametitle{Solving(a)}
    \item Given that 
    \begin{align}
        s&=\sum_{n=0}^N a_n x[n]\\
        s^2&=\sum_{n=0}^N a_n x[n]\sum_{n=0}^N a_n x[n]\\
        &=\sum_{n=0}^N a_n x[n]\sum_{m=0}^N a_m x[m]\\
        &=\sum_{n=0}^N\sum_{m=0}^Na_n a_m x[n]x[m]
    \end{align}
\end{frame}
\begin{frame}
    \begin{align}
        E\cbrak{s^2}&=\sum_{n=0}^N\sum_{m=0}^Na_n a_m E\cbrak{x[n]x[m]}
    \end{align}
    From,
     \begin{align}           E\cbrak{x[m_1]x[m_2]}&=R_x[m_1,m_2]\\
        E\cbrak{s^2}&=\sum_{n=0}^N\sum_{m=0}^Na_n a_m R_x[n,m]\\
       &=\sum_{n=0}^N\sum_{m=0}^Na_n a_m q[n]\delta[n - m]\\
        &=\sum_{n=0}^N a_n^2 q[n]
    \end{align}
\end{frame}

\begin{frame}
\frametitle{Solving(b)}
    \item Given that 
    \begin{align}
        s&=\int_0^T a\brak{t}x\brak{t}dt\\
        s^2&=\int_0^T a\brak{t}x\brak{t}dt\int_0^T a\brak{t}x\brak{t}dt\\
        &=\int_0^T a\brak{t}x\brak{t}dt\int_0^T a\brak{k}x\brak{k}dk\\
        &=\int_0^T\int_0^T a\brak{t}a\brak{k}x\brak{t}x\brak{k}dk dt 
    \end{align}
\end{frame}

\begin{frame}
    \begin{align}
        E\cbrak{s^2}&=\int_0^T\int_0^T a\brak{t}a\brak{k}E\cbrak{x\brak{t}x\brak{k}}dk dt
    \end{align}
    From,
     \begin{align}           E\cbrak{x\brak{t_1}x\brak{t_2}}&=R_x\brak{t_1,t_2}\\
     E\cbrak{s^2}&=\int_0^T\int_0^T a\brak{t}a\brak{k}R_x\brak{t_1,t_2}dk dt\\
     &=\int_0^T\int_0^T a\brak{t}a\brak{k}q\brak{t}\delta\brak{t-k}dk dt\\
     &=\int_0^Ta^2\brak{t}q\brak{t}dt
    \end{align}
    Hence proved.
\end{frame}
\end{enumerate}
\end{document}